theories/Plugin.v
@@ -2,5 +2,6 @@ Require Import Vector.
 Require Import Circuit.
 
 Register le_S as num.nat.le_S.
+Register length as core.list.length.
 
 Declare ML Module "vcpu_plugin:vcpu-plugin.plugin".
